Bisimilarity.v

theories/Bisimilarity.v
@@ -1,38 +1,47 @@
-Require Import MEBI.Examples.CADP.
-
 (* https://rocq-prover.org/doc/v8.9/stdlib/Coq.Relations.Relation_Operators.html *)
-Require Import Coq.Relations.Relation_Definitions.
-Require Import Coq.Relations.Relation_Operators.
-Require Coq.Relations.Operators_Properties.
-Require Import Coq.Classes.RelationClasses.
+Require Import Relation_Definitions.
+Require Import Relation_Operators.
 
 Set Primitive Projections.
 
-(**************************************)
 Section Definitions.
   Context (M : Type) (A : Type).
-  (* option A = None -> silent (tau-labelled) transition *)
   Definition LTS : Type := M -> option A -> M -> Prop.
   (* tau-labelled transition *)
-  Definition tau (R : LTS) : relation M := fun (x y : M) => R x None y.
+  Definition tau (R : LTS) : relation M := fun x y => R x None y.
 End Definitions.
 Arguments tau {M A} R.
 
-(**************************************)
+Hint Constructors clos_refl_trans_1n clos_trans_1n : rel_db.
+Lemma clos_t_clos_rt {A : Type} (R : relation A) :
+      forall x y, clos_trans_1n A R x y -> clos_refl_trans_1n A R x y.
+Proof. intros x y H; induction H; eauto with rel_db. Qed.
+
+Lemma clos_rt_clos_t {A : Type} {R : relation A} :
+      forall {x y z}, R x y -> clos_refl_trans_1n A R y z ->
+                    clos_trans_1n A R x z.
+Proof. intros x y z Rxy H. revert x Rxy. induction H; eauto with rel_db. Qed.
+
+Hint Resolve clos_t_clos_rt clos_rt_clos_t : rel_db.
+
 Section WeakTrans.
   Context {M : Type} {A : Type} (lts : LTS M A).
 
   (* trace of tau-labelled transitions *)
-  Definition silent  : relation M := clos_refl_trans_1n M (tau lts).
+  Definition silent : relation M := clos_refl_trans_1n M (tau lts).
   Definition silent1 : relation M := clos_trans_1n M (tau lts).
 
-  (* x ==> pre_str ->^a post_str ==> y *)
+  (*  x ==> pre_str ->^a post_str ==> y *)
   Record weak_tr (x z : M) a (t y : M) : Prop :=
     Pack_weak { pre : silent x z; str : lts z a t; post : silent t y }.
-  Definition weak (x : M) a (y : M) : Prop := exists z t, weak_tr x z a t y.
+  Definition weak (x : M) a (y : M) : Prop :=
+    exists z t, weak_tr x z a t y.
 End WeakTrans.
+Hint Constructors weak_tr : rel_db.
+Hint Resolve pre post : rel_db.
+Hint Unfold silent silent1 weak : rel_db.
 
-(**************************************)
+
 Section WeakSim.
   Context {M : Type} {N : Type} {A : Type} (ltsM : LTS M A) (ltsN : LTS N A).
 
@@ -42,303 +51,96 @@ Section WeakSim.
           weak ltsM m1 (Some a) m2 ->
           exists n2, weak ltsN n1 (Some a) n2 /\ G m2 n2;
         sim_tau : forall m2,
-          (* weak ltsM m1 None m2 -> *)
+          (*  weak ltsM m1 None m2 -> *)
           silent1 ltsM m1 m2 ->
           exists n2, silent ltsN n1 n2 /\ G m2 n2;
       }.
 
-  CoInductive weak_sim (s : M) (t : N) : Prop := 
-    In_sim { out_sim : simF weak_sim s t }.
+  CoInductive weak_sim (s : M) (t : N) : Prop
+    := In_sim { out_sim :  simF weak_sim s t }.
 End WeakSim.
+Arguments Pack_sim {M N A}%_type_scope & {ltsM ltsN G}%_function_scope
+  {m1 n1} (sim_weak sim_tau)%_function_scope.
+Arguments sim_weak {M N A}%_type_scope & {ltsM ltsN G%_function_scope m1 n1} s
+  {m2 a} _.
+Arguments sim_tau {M N A}%_type_scope & {ltsM ltsN G%_function_scope m1 n1} s
+  {m2} _.
+Hint Constructors simF : rel_db.
+Hint Constructors weak_sim : rel_db.
+Hint Resolve sim_weak sim_tau : rel_db.
 
-(** (unused) **************************)
-Lemma _weak_sim_silent_refl (X A : Type) (lts : LTS X A)
-: forall x, weak_sim lts lts x x -> silent lts x x.
-Proof. intros x Hxx. constructor. Qed.
+Ltac needs_weak_simpl ltsR x a :=
+  match goal with
+  | [ H : @weak _ _ ltsR x a _ |- _ ] => fail 1
+  | |- _ => idtac
+  end.
 
-(** (unused) **************************)
-Lemma _weak_sim_silent_geq_1 (X A : Type) (lts : LTS X A)
-: forall x, weak_sim lts lts x x -> silent lts x x ->
-  exists y, silent1 lts x y -> silent lts x y /\ weak_sim lts lts x y.
-Proof. 
-  intros x Hxx_sim Hxx. eexists x. intros _. split.
-  - apply Hxx.
-  - apply Hxx_sim. 
-Qed.
+Ltac needs_silent_simpl ltsM ltsN x y :=
+  unfold silent, silent1, tau in *;
+  match goal with
+  | [ H : @clos_trans_1n _ (fun a b => ltsM a None b) x ?y
+    , W : @weak_sim _ _ _ ltsM ltsN ?y y
+    |- _ ]
+      => fail 1
+  | [ H : @clos_trans_1n _ (fun a b => ltsN a None b) y _ |- _ ]
+      => fail 1
+  | |- _ => idtac
+  end.
 
-(** (unused) **************************)
-Lemma _silent_geq_1 (X A : Type) (lts : LTS X A)
-: forall x, silent lts x x ->
-  exists y, silent1 lts x y -> silent lts x y.
-Proof. intros x Hxx. eexists x. intros _. apply Hxx. Qed.
+Ltac bisim_simpl :=
+  unfold silent, silent1, tau in *;
+  repeat match goal with
+  | [ H : _ /\ _ |- _] => destruct H
+  | [ H : exists _, _ |- _ ] => destruct H
+  | [ H : @simF _ _ _ ?ltsM ?ltsR _ ?m ?n, W : @weak _ _ ?ltsM ?m ?a _ |- _] =>
+    needs_weak_simpl ltsR n a;
+    destruct (@sim_weak _ _ _ _ _ _ _ _ H _ _ W) as [?[??]]
+  | [ H : @simF _ _ _ ?ltsM ?ltsN _ ?m ?n
+    , T : @clos_trans_1n _ (fun a b => ?ltsM a None b) ?m _
+    |- _ ] =>
+      needs_silent_simpl ltsM ltsN m n;
+      let Th := fresh "Th" in
+      let Tt := fresh "Tt" in
+      destruct (@sim_tau _ _ _ _ _ _ _ _ H _ T) as [?[[|?? Th Tt]?]];
+      [|pose proof (@clos_rt_clos_t _ _ _ _ _ Th Tt)]
+  end.
 
-(** (unused) **************************)
-Lemma _tau_silent1 (X A: Type) (lts : LTS X A)
-: forall x y, tau lts x y -> silent1 lts x y.
-Proof. intros x y Hxy. constructor. apply Hxy. Qed.
+Hint Extern 0 => progress bisim_simpl : rel_db.
 
-(** (1 admitted case) *****************)
-Lemma silent1_step (X A: Type) (lts : LTS X A)
-: forall x y, silent1 lts x y -> silent lts x y.
-Proof.
-  intros x y Hxy. induction Hxy.
-  - eapply rt1n_trans. apply H. apply rt1n_refl.
-  - apply (rt1n_trans _ _ _ _ _ H IHHxy).
-Qed.
+Ltac bisim_cofix :=
+  let CH := fresh "CH" in
+  cofix CH; intros; constructor;
+  (repeat match goal with
+         | [ H : @weak_sim _ _ _ _ _ _ _ |- _ ] => apply out_sim in H
+         end).
+Tactic Notation "solve_bisim" integer(t) := bisim_cofix; eauto t with rel_db.
 
-(** (depends on Lemma [silent1_step]) *)
-Lemma weak_sim_refl (X A : Type) (lts : LTS X A)
-: forall x, weak_sim lts lts x x.
-Proof.
-  cofix CH; intros x. 
-  (* cofix Hxx_sim. *)
-  apply In_sim. apply Pack_sim.
-  { intros y a Hxy; eexists y; split.
-    - apply Hxy.
-    - apply CH. Guarded. }
-  { intros y Hxy.
-    eexists y. split; [| apply CH]. Guarded.
-    (*****************************)
-    (* silent  ltsX x y       -> *)
-    (* silent1 ltsX x y          *)
-    (*****************************)
-    apply silent1_step. apply Hxy. }
-Qed.
+Lemma weak_sim_refl {M A} (lts : LTS M A) : forall x, weak_sim lts lts x x.
+Proof. solve_bisim 8. Qed.
+Hint Resolve weak_sim_refl : rel_db.
 
-(**************************************)
-(* Lemma silent_trans_l (X A : Type) (lts : LTS X A)
-: forall x y, silent1 lts x y -> 
-  exists z, silent lts x z -> silent1 lts z y.
-Proof.
-  intros x y Hxy. apply clos_t1n_trans in Hxy.
-  inversion  Hxy as [|z]; subst.
-  - eexists x. intros Hxx. apply clos_trans_t1n. apply Hxy.
-  - eexists z. intros Hxz. apply clos_trans_t1n. apply H0.
-Qed.
+Lemma weak_sim_trans {M N R A}
+  (ltsM : LTS M A) (ltsN : LTS N A) (ltsR : LTS R A)
+  : forall x y r, weak_sim ltsM ltsN x y -> weak_sim ltsN ltsR y r ->
+                  weak_sim ltsM ltsR x r.
+Proof. solve_bisim 19. Qed.
+Hint Immediate weak_sim_trans : rel_db.
 
-(**************************************)
-Lemma silent_trans_r (X A : Type) (lts : LTS X A)
-: forall x y, silent1 lts x y -> 
-  exists z, silent1 lts x z -> silent lts z y.
-Proof. intros x y Hxy. eexists y. intros _. constructor. Qed.
-
-(** (unused, 1 admitted case) *********)
-Lemma _silent_trans (X A : Type) (lts : LTS X A)
-: forall x, weak_sim lts lts x x -> 
-  forall y, silent1 lts x y -> 
-  exists z1 z2, silent lts x z1 -> silent1 lts z1 z2 -> silent lts z2 y.
-Proof.
-  intros x Hxx_sim y Hxy.
-
-  assert (Hxy_z := Hxy); apply silent_trans_l in Hxy_z.
-  destruct Hxy_z as [z1 Hxy_z]; eexists z1.
-  apply silent_trans_r in Hxy_z.
-  { destruct Hxy_z as [z2 Hxy_z]; eexists z2.
-    intros Hxz Hzz. apply Hxy_z. apply Hzz. }
-  { (********************************)
-    (* Hxy : silent1 lts x y        *)
-    (* apply silent_trans_l in Hxy. *)
-    About silent_trans_l.
-    (* Hxy : silent lts x z1 ->     *)
-    (*       silent lts z1 y        *)
-    (* apply silent_trans_r in Hxy. *)
-    About silent_trans_r.
-    (* Hxy : silent lts x z1   ->   *)
-    (*       silent1 lts z1 z2 ->   *)
-    (*       silent lts z2 y        *)
-    (********************************)
-    admit. }
-Admitted. *)
-
-Lemma rt_t {X A : Type} {ltsX : LTS X A}
-: forall {x1 x2 x3},
-  tau ltsX x1 x2 ->
-  clos_refl_trans_1n X (tau ltsX) x2 x3 ->
-  clos_trans_1n X (tau ltsX) x1 x3.
-Proof.
-  intros x y z Hxy Hyz.
-  revert x Hxy.
-  induction Hyz.
-  - intros x0 Hxy. eapply t1n_step, Hxy.
-  - intros x0 Hxy.  
-    eapply t1n_trans.
-    + apply Hxy.
-    + apply IHHyz. apply H.   
-Qed.
-
-(** (1 admitted case) *****************)
-Lemma weak_sim_trans (X Y Z A : Type) 
-(ltsX : LTS X A) (ltsY : LTS Y A) (ltsZ : LTS Z A) 
-: forall x y z,
-  weak_sim ltsX ltsY x y -> 
-  weak_sim ltsY ltsZ y z -> 
-  weak_sim ltsX ltsZ x z.
-Proof.
-  cofix CH; intros x1 y1 z1.
-  intros Hxy. intros Hyz.
-
-  inversion Hxy as [Hxy_inv]; subst; destruct Hxy_inv as [Hxy_weak Hxy_tau].
-  inversion Hyz as [Hyz_inv]; subst; destruct Hyz_inv as [Hyz_weak Hyz_tau].
-
-  apply In_sim. apply Pack_sim.
-  { intros x2 ax Hx. 
-  
-    apply Hxy_weak in Hx; inversion_clear Hx as [y2 Hy_xy]; subst.
-    destruct Hy_xy as [Hy Hxy2].
-
-    apply Hyz_weak in Hy; inversion_clear Hy as [z2 Hz_yz]; subst.
-    destruct Hz_yz as [Hz Hyz2].
-
-    eexists z2. split.
-    - apply Hz.
-    - About CH. apply (@CH x2 y2 z2 Hxy2 Hyz2). Guarded. }
-  { intros x2 Hx.
-  
-    apply Hxy_tau in Hx. destruct Hx as [y2 [[|y2a y2b Hy12a] H0]].
-    - eexists z1. split.
-      + apply rt1n_refl.
-      + eapply CH. apply H0. apply Hyz. Guarded.
-    - (* turn into lemma *)
-
-      About rt_t.
-      apply (rt_t Hy12a) in H.
-      apply Hyz_tau in H. destruct H as [z2 [Hzz Hyz2]].
-      eexists z2. split.
-      apply Hzz. eapply CH. apply H0. apply Hyz2. Guarded.
-  } 
-Qed.
-
-(**************************************)
 Section WeakBisim.
   Context {M : Type} {N : Type} {A : Type} (ltsM : LTS M A) (ltsN : LTS N A).
 
   Definition weak_bisim (s : M) (t : N) : Prop
     := weak_sim ltsM ltsN s t /\ weak_sim ltsN ltsM t s.
 End WeakBisim.
+Hint Unfold weak_bisim : rel_db.
 
-(**************************************)
-Lemma weak_bisim_refl (M A : Type) (ltsM : LTS M A)
-: forall m, weak_bisim ltsM ltsM m m.
-Proof. constructor 1; try apply weak_sim_refl. Qed.
+Lemma wk_bisim_refl {M A} (lts : LTS M A) : forall x, weak_bisim lts lts x x.
+Proof. eauto with rel_db. Qed.
 
-(**************************************)
-Lemma weak_bisim_sym (X Y A : Type) (ltsX : LTS X A) (ltsY : LTS Y A) 
-: forall x y, weak_bisim ltsX ltsY x y -> weak_bisim ltsY ltsX y x.
-Proof. 
-  intros x y Hxy. split.
-  - destruct Hxy as [_ Hyx]. apply Hyx.
-  - destruct Hxy as [Hxy _]. apply Hxy.
-Qed.
+Lemma wk_bisim_trans {M A} (lts : LTS M A) : forall x y z,
+    weak_bisim lts lts x y -> weak_bisim lts lts y z -> weak_bisim lts lts x z.
+Proof. eauto with rel_db. Qed.
 
-(**************************************)
-Lemma weak_bisim_trans (X Y Z A : Type) 
-(ltsX : LTS X A) (ltsY : LTS Y A) (ltsZ : LTS Z A) 
-: forall x y z,
-  weak_bisim ltsX ltsY x y ->
-  weak_bisim ltsY ltsZ y z ->
-  weak_bisim ltsX ltsZ x z.
-Proof.
-  intros x y z Hbxy Hbyz.
-  destruct Hbxy as [Hsxy Hsyx]. destruct Hbyz as [Hsyz Hszy].
-  split. 
-  - apply (@weak_sim_trans X Y Z A ltsX ltsY ltsZ x y z).
-    + apply Hsxy.
-    + apply Hsyz.
-  - apply (@weak_sim_trans Z Y X A ltsZ ltsY ltsX z y x).
-    + apply Hszy.
-    + apply Hsyx.
-Qed.
-
-(**************************************)
-Module BisimTest1.
-  Inductive action : Type := | TheAction1 | TheAction2.
-
-  Inductive term : Type :=
-    | trec : term
-    | tend : term
-    | tfix : term -> term
-    | tact : option action -> term -> term
-    | tpar : option action -> option action -> term -> term
-    .
-
-  Fixpoint subst (t1 : term) (t2 : term) :=
-    match t2 with
-    | trec => t1
-    | tend => tend
-    | tfix t => tfix t
-    | tact a t => tact a (subst t1 t)
-    | tpar a b t => tpar a b (subst t1 t)
-    end.
-
-  Inductive termLTS : term -> option action -> term -> Prop :=
-    | do_act : forall a t, 
-        (* out_sim (tact a t) = consF a t -> *)
-        termLTS (tact a t) a t
-
-    | do_parl : forall a b t, 
-        (* out_sim (tpar a b t) = consF a (tact b t) -> *)
-        termLTS (tpar a b t) a (tact b t)
-
-    | do_parr : forall a b t, 
-        (* out_sim (tpar a b t) = consF a (tact a t) -> *)
-        termLTS (tpar a b t) b (tact a t)
-
-    | do_fix : forall a t t',
-        (* out_sim (tfix t) = consF a t' -> *)
-        termLTS (subst (tfix t) t) a t' ->
-        termLTS (tfix t) a t'
-    .
-
-  Inductive termLTS_tc : term -> Prop :=
-    | do_step : forall t a t', termLTS t a t' -> termLTS_tc t' -> termLTS_tc t
-    | do_none : forall t, termLTS_tc t
-    .
-
-  Lemma sim_tend : weak_sim termLTS termLTS (tend) (tend).
-  Proof. apply weak_sim_refl. Qed.
-End BisimTest1.
-
-(**************************************)
-Module BisimExa1. Import BisimTest1.
-
-  Example m1 := (tact None (tact (Some TheAction1) (tact None tend))).
-  Example n1 := (tact (Some TheAction1) tend).
-
-  Goal weak_sim termLTS termLTS m1 n1.
-  Proof. 
-    apply In_sim. apply Pack_sim.
-    { intros m2 a Hw. destruct Hw. destruct H. destruct H.
-      destruct pre0.
-      inversion str0.
-      inversion H; subst. 
-      destruct pre0; [| inversion H0]. (* clear H. *)
-      inversion str0; subst. (* clear str0. *)
-      inversion post0; subst.
-      - eexists tend. split.
-        + do 2 eexists. do 2 constructor. 
-        + admit.
-      - eexists tend. split.
-        + do 2 eexists. do 2 constructor.
-        + admit.
-    }
-    { intros m2 Hw. eexists n1. split.
-      - constructor.
-      - admit. 
-    }
-  Admitted. 
-End BisimExa1.
-
-(**************************************)
-Module BisimExa2. Import BisimTest1.
-  Example m1 := (tfix (tact (Some TheAction1) trec)).
-  Example n1 := (tact (Some TheAction1) (tfix (tact (Some TheAction1) trec))).
-  
-  Goal weak_sim termLTS termLTS m1 n1.
-  Proof.
-    apply In_sim; apply Pack_sim.
-  
-  Admitted.
-
-End BisimExa2.
-
-
+Lemma wk_bisim_sym {M A} (lts : LTS M A) : forall x y,
+    weak_bisim lts lts x y -> weak_bisim lts lts y x.
+Proof. eauto with rel_db. Qed.
